theories/LanguagesUtils.v
@@ -1,0 +1,54 @@
+From Coq Require Import Nat.
+
+From Coq Require Import List.
+
+Search (nat).
+
+Inductive variable : Type :=
+  | X : nat -> variable  (* input  *)
+  | Z : nat -> variable  (* local  *)
+  | Y : variable.        (* output *)
+
+Inductive label : Type :=
+  | A : nat -> label.
+
+
+Definition eqb_var v1 v2 := 
+  match v1, v2 with 
+  | X a, X b => a =? b
+  | Z a, Z b => a =? b
+  | Y, Y  => true
+  | _, _ => false
+  end.
+
+Definition eqb_lbl l1 l2 :=
+  match l1, l2 with 
+  | A a, A b => a =? b
+  end.
+
+Theorem eqb_var_refl : forall v, eqb_var v v = true.
+Proof.
+  destruct v; try (apply PeanoNat.Nat.eqb_refl); reflexivity.
+Qed.
+
+Theorem var_eqb_eq : forall v1 v2 : variable, eqb_var v1 v2 = true <-> v1 = v2.
+Proof.
+  intros v1 v2. split; intros H.
+  (* -> *) 
+  destruct v1; destruct v2; (try discriminate).
+  - simpl in H. rewrite PeanoNat.Nat.eqb_eq in H. rewrite H. reflexivity.
+  - simpl in H. rewrite PeanoNat.Nat.eqb_eq in H. rewrite H. reflexivity.
+  - reflexivity.
+  (* <- *)
+  - rewrite H. apply eqb_var_refl.
+Qed.
+
+Theorem var_eqb_neq : forall v1 v2 : variable, eqb_var v1 v2 = false <-> v1 <> v2.
+Proof.
+  intros v1 v2. split; intros H.
+  - intros H1. rewrite H1 in H. rewrite eqb_var_refl in H. discriminate.
+  - unfold not in H. destruct (eqb_var v1 v2) eqn:Heq.
+    + apply var_eqb_eq in Heq. contradiction. 
+    + reflexivity.
+Qed.
+
